Fix some proofs from the previous change

Wavelet/Compile/AffineOp.lean
@@ -34,7 +34,7 @@ inductive Expr.AffineInrOp
       AffineInrOp used₁ left →
       AffineInrOp used₂ right →
       used₁.Disjoint used₂ →
-      AffineInrOp (used₁ ++ used₂) (.br cond left right)
+      AffineInrOp (used₁ ++ used₂) (.br c left right)
 
 def Fn.AffineInrOp [Arity Op₁] [Arity Op₂]
   (fn : Fn (Op₁ ⊕ Op₂) χ V m n) : Prop :=
@@ -100,10 +100,11 @@ namespace Wavelet.Compile
 
 open Semantics Seq Dataflow Fn
 
+/- TODO: Fix proof performance -/
+set_option maxHeartbeats 500000
+
 /--
 `compileExpr` preserves `AffineInrOp`.
-
-TODO: Proof performance
 -/
 theorem compile_expr_preserves_aff_op
   [Arity Op₁] [Arity Op₂]
@@ -114,70 +115,84 @@ theorem compile_expr_preserves_aff_op
   (haff : expr.AffineInrOp usedOps) :
     (compileExpr (V := V) definedVars pathConds expr).AffineInrOp usedOps
   := by
-  sorry
   -- induction expr generalizing definedVars pathConds usedOps with
-  -- | ret =>
-  --   simp [compileExpr, AtomicProcs.AffineInrOp,
-  --     AtomicProc.forwardc, AtomicProc.sink]
-  --   -- grind only [= Vector.toArray_map, = List.getElem_cons, = Vector.toArray_empty,
-  --   --   → Array.eq_empty_of_map_eq_empty, =_ Vector.toList_toArray, = List.length_nil,
-  --   --   = List.length_cons, cases Or]
-  --   sorry
-  -- | tail =>
-  --   simp [compileExpr, AtomicProcs.AffineInrOp,
-  --     AtomicProc.forwardc, AtomicProc.sink]
-  --   -- grind only [= Vector.toArray_map, = List.getElem_cons, = Vector.toArray_empty,
-  --   --   → Array.eq_empty_of_map_eq_empty, =_ Vector.toList_toArray, = List.length_nil,
-  --   --   = List.length_cons, cases Or]
-  --   sorry
-  -- | op o args rets cont ih =>
-  --   cases o with
-  --   | inl op₁ =>
-  --     cases haff with | aff_op_inl haff =>
-  --     simp [compileExpr]
-  --     -- grind only [= List.getElem_cons, = List.mem_cons, =_ Vector.toList_toArray,
-  --     --   = List.length_cons, AtomicProcs.AffineInrOp, usr List.length_pos_of_mem,
-  --     --   usr List.getElem_mem, usr List.eq_or_mem_of_mem_cons, cases Or]
-  --     sorry
-  --   | inr op₂ =>
-  --     cases haff with | aff_op_inr hnot_mem haff =>
-  --     simp [compileExpr]
-  --     -- grind only [= List.getElem_cons, = List.mem_cons, = List.getElem_cons_zero,
-  --     --   =_ Vector.toList_toArray, = List.length_cons, AtomicProcs.AffineInrOp,
-  --     --   usr List.length_pos_of_mem, usr List.getElem_mem, usr List.eq_or_mem_of_mem_cons, cases Or]
-  --     sorry
-  -- | br cond left right ih₁ ih₂ =>
-  --   cases haff with | aff_br haff₁ haff₂ hdisj
-  --   simp [compileExpr, AtomicProcs.AffineInrOp, compileExpr.branchMerge]
-  --   constructor
-  --   · intros _ _ _ hop
-  --     -- grind only [usr List.length_filter_le, = List.removeAll_nil, = List.removeAll_cons,
-  --     --   =_ List.countP_eq_length_filter, = Vector.length_toList, =_ Vector.toList_toArray,
-  --     --   AtomicProc.switch, = Vector.append_assoc_symm, = Vector.toArray_cast, = List.length_cons,
-  --     --   = Vector.toList_mk, AtomicProcs.AffineInrOp, AtomicProc.fork, usr List.length_pos_of_mem,
-  --     --   = List.size_toArray, = Vector.toArray_append, = Vector.append_assoc, AtomicProc.merge]
-  --     sorry
-  --   · intros i j depOp inputs outputs depOp' inputs' outputs'
-  --       hne hi hj hget_i hget_j
-  --     sorry
-  --     -- simp [List.getElem_cons, List.getElem_append] at hget_i hget_j hi hj
-  --     -- split_ifs at hget_i
-  --     -- any_goals simp [AtomicProc.switch, AtomicProc.merge, AtomicProc.fork] at hget_i
-  --     -- any_goals omega
-  --     -- all_goals
-  --     --   split_ifs at hget_j
-  --     --   any_goals simp [AtomicProc.switch, AtomicProc.merge, AtomicProc.fork] at hget_j
-  --     --   any_goals omega
-  --     -- · exact (ih₁ haff₁).2 (by omega) (by omega) (by omega) hget_i hget_j
-  --     -- · intros h; subst h
-  --     --   have h₁ := (ih₁ haff₁).1 (List.mem_of_getElem hget_i)
-  --     --   have h₂ := (ih₂ haff₂).1 (List.mem_of_getElem hget_j)
-  --     --   exact False.elim (hdisj h₁ h₂)
-  --     -- · intros h; subst h
-  --     --   have h₁ := (ih₁ haff₁).1 (List.mem_of_getElem hget_j)
-  --     --   have h₂ := (ih₂ haff₂).1 (List.mem_of_getElem hget_i)
-  --     --   exact False.elim (hdisj h₁ h₂)
-  --     -- · exact (ih₂ haff₂).2 (by omega) (by omega) (by omega) hget_i hget_j
+  cases expr with
+  | ret =>
+    simp [compileExpr, AtomicProcs.AffineInrOp,
+      AtomicProc.forwardc, AtomicProc.sink]
+    grind only [= Vector.toArray_map, = List.getElem_cons, = Vector.toArray_empty,
+      → Array.eq_empty_of_map_eq_empty, =_ Vector.toList_toArray, = List.length_nil,
+      = List.length_cons, cases Or]
+  | tail =>
+    simp [compileExpr, AtomicProcs.AffineInrOp,
+      AtomicProc.forwardc, AtomicProc.sink]
+    grind only [= Vector.toArray_map, = List.getElem_cons, = Vector.toArray_empty,
+      → Array.eq_empty_of_map_eq_empty, =_ Vector.toList_toArray, = List.length_nil,
+      = List.length_cons, cases Or]
+  | op o args rets cont =>
+    cases o with
+    | inl op₁ =>
+      cases haff with | aff_op_inl haff =>
+      simp [compileExpr]
+      have ih := compile_expr_preserves_aff_op
+        (V := V) (expr := cont)
+        (definedVars := definedVars.removeAll args.toList ++ rets.toList)
+        (pathConds := pathConds)
+        haff
+      grind only [= List.getElem_cons, = List.mem_cons, =_ Vector.toList_toArray,
+        = List.length_cons, AtomicProcs.AffineInrOp, usr List.length_pos_of_mem,
+        usr List.getElem_mem, usr List.eq_or_mem_of_mem_cons, cases Or]
+    | inr op₂ =>
+      cases haff with | aff_op_inr hnot_mem haff =>
+      have ih := compile_expr_preserves_aff_op
+        (V := V) (expr := cont)
+        (definedVars := definedVars.removeAll args.toList ++ rets.toList)
+        (pathConds := pathConds)
+        haff
+      simp [compileExpr]
+      grind only [= List.getElem_cons, = List.mem_cons, = List.getElem_cons_zero,
+        =_ Vector.toList_toArray, = List.length_cons, AtomicProcs.AffineInrOp,
+        usr List.length_pos_of_mem, usr List.getElem_mem, usr List.eq_or_mem_of_mem_cons, cases Or]
+  | br c left right =>
+    cases haff with | aff_br haff₁ haff₂ hdisj
+    simp [compileExpr, AtomicProcs.AffineInrOp, compileExpr.branchMerge]
+    have ih₁ := compile_expr_preserves_aff_op
+      (V := V) (expr := left)
+      (definedVars := definedVars.removeAll [c])
+      (pathConds := (true, .var c pathConds) :: pathConds)
+      haff₁
+    have ih₂ := compile_expr_preserves_aff_op
+      (V := V) (expr := right)
+      (definedVars := definedVars.removeAll [c])
+      (pathConds := (false, .var c pathConds) :: pathConds)
+      haff₂
+    constructor
+    · intros _ _ _ hop
+      grind only [usr List.length_filter_le, = List.removeAll_nil, = List.removeAll_cons,
+        =_ List.countP_eq_length_filter, = Vector.length_toList, =_ Vector.toList_toArray,
+        AtomicProc.switch, = Vector.append_assoc_symm, = Vector.toArray_cast, = List.length_cons,
+        = Vector.toList_mk, AtomicProcs.AffineInrOp, AtomicProc.fork, usr List.length_pos_of_mem,
+        = List.size_toArray, = Vector.toArray_append, = Vector.append_assoc, AtomicProc.merge]
+    · intros i j depOp inputs outputs depOp' inputs' outputs'
+        hne hi hj hget_i hget_j
+      simp [List.getElem_cons, List.getElem_append] at hget_i hget_j hi hj
+      split_ifs at hget_i
+      any_goals simp [AtomicProc.switch, AtomicProc.merge, AtomicProc.fork] at hget_i
+      any_goals omega
+      all_goals
+        split_ifs at hget_j
+        any_goals simp [AtomicProc.switch, AtomicProc.merge, AtomicProc.fork] at hget_j
+        any_goals omega
+      · exact ih₁.2 (by omega) (by omega) (by omega) hget_i hget_j
+      · intros h; subst h
+        have h₁ := ih₁.1 (List.mem_of_getElem hget_i)
+        have h₂ := ih₂.1 (List.mem_of_getElem hget_j)
+        exact False.elim (hdisj h₁ h₂)
+      · intros h; subst h
+        have h₁ := ih₁.1 (List.mem_of_getElem hget_j)
+        have h₂ := ih₂.1 (List.mem_of_getElem hget_i)
+        exact False.elim (hdisj h₁ h₂)
+      · exact ih₂.2 (by omega) (by omega) (by omega) hget_i hget_j
 
 /-- `compileFn` preserves `AffineInrOp`. -/
 theorem compile_fn_preserves_aff_op
